

Discrete Test 2 Review: Answers!

5

- (1) Prove $\forall a, b \in \mathbb{Z}$, if $(a \bmod 6 = 5 \text{ and } b \bmod 4 = 3)$ then $4a + 6b \bmod 8 = 6$.
Use a Direct proof.

a) Write the assumption, translated to algebraic equations.

$$\boxed{a = 6m + 5 \quad \text{and} \quad b = 4k + 3}$$

b) Write what we want to show, translated to algebraic equations.

$$\boxed{4a + 6b = 8p + 6}$$

c) Write the proof steps.

$$\begin{aligned} 4a + 6b &= 4(6m + 5) + 6(4k + 3) \\ &= 24m + 20 + 24k + 18 \\ &= 24m + 24k + 32 + 6 \\ &= \boxed{8(3m + 3k + 4) + 6} \end{aligned}$$

- (2) Suppose we were to prove the statement " $\forall y \in \mathbb{Z}$, y is even $\Rightarrow (y^3 - 1)$ is odd." (Answer using algebraic equations, without using the word "not" or the symbol " \sim ".)

a) For a direct proof we assume $y = 2k$ and show $y^3 - 1 = 2m + 1$.

b) For proof using the contrapositive we assume $y^3 - 1 = 2p$ and show $y = 2q + 1$.

c) For proof by contradiction we assume $y = 2k$ and $y^3 - 1 = 2m$ and show that we reach a false conclusion.

- (3) Use contradiction to prove: $\forall a, b \in \mathbb{Z}$, if a is even and b is odd then 4 does not divide $(a^2 + 2b^2)$.

a) Negate the statement.

$$\boxed{\exists a, b \in \mathbb{Z} \text{ s.t. } a \text{ is even and } b \text{ is odd and } 4 \mid (a^2 + 2b^2).}$$

b) What do we assume? Translate to algebraic equations.

$$\boxed{a = 2k} \quad \text{and} \quad \boxed{b = 2m + 1} \quad \text{and} \quad \boxed{a^2 + 2b^2 = 4p}$$

c) Use the assumptions to prove that $4 \nmid 2$, as an algebraic equation.

$$\begin{aligned} a^2 + 2b^2 &= 4p \\ \Rightarrow (2k)^2 + 2(2m + 1)^2 &= 4p \\ \Rightarrow 4k^2 + 2(4m^2 + 4m + 1) &= 4p \\ &\Rightarrow 4(k^2 + 2m^2 + 2m) + 2 = 4p \\ &\Rightarrow 4p - 4(k^2 + 2m^2 + 2m) = 2 \\ &\Rightarrow \boxed{4(p - k^2 - 2m^2 - 2m) = 2} \end{aligned}$$

□

- (4) Prove by induction that: $\forall n \in \mathbb{N}$, if $n \geq 2$ then $3|(2^{(4n-4)} + 2^{(2n-3)})$.
a) Show the base case.

$$\text{Base case: } n = 2 : 2^4 + 2^1 = 18 = 3(6).$$

- b) State the induction assumption, translate to algebraic equations.

$$2^{(4k-4)} + 2^{(2k-3)} = 3m.$$

- c) State what we need to show, translate to algebraic equations.

$$2^{(4(k+1)-4)} + 2^{(2(k+1)-3)} = 3q$$

- d) Do the proof steps.

Proof.

$$2^{(4(k+1)-4)} + 2^{(2(k+1)-3)} = 16(2^{(4k-4)}) + 4(2^{(2k-3)})$$

$$= 15(2^{(4k-4)}) + 3(2^{(2k-3)}) + 2^{(4k-4)} + 2^{(2k-3)}$$

$$= 15(2^{(4k-4)}) + 3(2^{(2k-3)}) + 3m$$

$$= 3(5(2^{(4k-4)}) + 2^{(2k-3)} + m).$$

□

- (5) Use a Direct proof to prove: $\forall z \in \mathbb{Z}, 3|(z+1) \Rightarrow z^2 \pmod 3 = 1$.
a) Write the assumption, translated to algebraic equations.

$$z+1 = 3k$$

- b) Write what to show, translated to algebraic equations.

$$z^2 = 3m + 1$$

- c) Do the proof steps.

$$z^2 = (3k-1)^2$$

$$= 9k^2 - 6k + 1$$

$$= 3(3k^2 - 2k) + 1$$

□

For your use:

7

A	B	C	D	E	F	G	H	I	J	K	L	M	N	O	P	Q	R	S	T	U	V	W	X	Y	Z
1	2	3	4	5	6	7	8	9	10	11	12	13	14	15	16	17	18	19	20	21	22	23	24	25	26

- (6) Given the one-time-pad sequence (2, 6, 13, 1) encrypt the word COOL. Your output will be letters.

$$\begin{array}{rcl}
 C & = & 3 + 2 \\
 O & = & 15 + 6 \\
 O & = & 15 + 13 \\
 L & = & 12 + 1
 \end{array}
 \qquad
 \begin{array}{rcl}
 5 & \text{mod } 26 & = 5 \\
 21 & \text{mod } 26 & = 21 \\
 28 & \text{mod } 26 & = 2 \\
 13 & \text{mod } 26 & = 13
 \end{array}$$

E
U
B
M

- (7) Use the BBS sequence $a_n = (a_{n-1})^2 \text{ mod } pq$ to encrypt the word ZAP. Use the seed $a_0 = 11$ and the constant $pq = 7 * 13 = 91$. Start the encryption with $n = 1$.

$$\begin{array}{rcl}
 n & & a_n \\
 1 & Z = 26 + 30 & 56 \text{ mod } 26 = 4 \\
 2 & A = 1 + 81 & 82 \text{ mod } 26 = 4 \\
 3 & P = 16 + 9 & 25 \text{ mod } 26 = 25
 \end{array}$$

D
D
Y

$$\begin{array}{r}
 81^2 = 6561 \\
 91 \overline{) 6561} \text{ R } 9 \\
 \underline{637} \\
 191 \\
 \underline{182} \\
 9
 \end{array}$$

- (8) Use the same BBS sequence to decrypt the word LLJ. Use the seed $a_0 = 11$ and the constant $pq = 7 * 13 = 91$.

$$\begin{array}{rcl}
 L & = & 12 - 30 \\
 L & = & 12 - 81 \\
 J & = & 10 - 9
 \end{array}
 \qquad
 \begin{array}{rcl}
 -18 & \text{mod } 26 & = 8 \\
 -69 & \text{mod } 26 & = 9 \\
 1 & \text{mod } 26 & = 1
 \end{array}$$

H
I
A

- (9) Use the sequence $a_n = 5 + 3(a_{n-1} \text{ mod } n); a_0 = 7$ to encrypt the digits 1101. Start with $n = 1$.

$$\begin{array}{rcl}
 n & & a_n \\
 1 & 1 + 5 & 6 \text{ mod } 2 = 0 \\
 2 & 1 + 8 & 9 \text{ mod } 2 = 1 \\
 3 & 0 + 11 & 11 \text{ mod } 2 = 1 \\
 4 & 1 + 14 & 15 \text{ mod } 2 = 1
 \end{array}$$

0
1
1
1

- (10) Use the sequence $a_n = n^2 - 1$ to decrypt the digits 1110. Start with $n = 1$.

$$\begin{array}{rcl}
 n & & a_n \\
 1 & 1 + 0 & 1 \text{ mod } 2 = 1 \\
 2 & 1 + 3 & 4 \text{ mod } 2 = 0 \\
 3 & 1 + 8 & 9 \text{ mod } 2 = 1 \\
 4 & 0 + 15 & 15 \text{ mod } 2 = 1
 \end{array}$$

1
0
1
1

(11) Given universe $U = \{1, 2, 3, 4, 5, 7, 9, 10, 21, 25\}$; $A = \{7, 9, 10, 21, 25\}$; and $B = \{5, 4, 7, 10, 21\}$. Find the following:

$$\bullet \overline{A \cup B} = \bar{A} \cap \bar{B} = \bar{A} \cap B = B - A = \boxed{\{5, 4\}}$$

$$\bullet (A - B) \cup (B - A) = \{9, 25\} \cup \{5, 4\} = \boxed{\{9, 25, 5, 4\}}$$

$$\bullet \overline{(B - A) \cap A} = \overline{(B - A)} \cup \bar{A} = (B - A) \cup \bar{A} \\ = \{5, 4\} \cup \{1, 2, 3, 4, 5\} = \boxed{\{5, 4, 1, 2, 3\}}$$

$$\bullet |\mathcal{P}(A)| = 2^5 = \boxed{32}$$

$$\bullet |\mathcal{P}(A \times B) \times A| = |\mathcal{P}(A \times B)| \cdot |A| = 2^{|A \times B|} \cdot 5 = 2^{5 \cdot 5} \cdot 5 = \boxed{5(2^{25})}$$

$$\bullet |\mathcal{P}(A \cup B)| = |\mathcal{P}(\{5, 4, 7, 9, 10, 21, 25\})| = \boxed{2^7}$$

$$\bullet |\overline{A \cup B}| = |\{1, 2, 3\}| = \boxed{3}$$